decomposition axiom moved + serious refactoring + axioms weakening + adjusted MiniML

refocusing_lang.v
@@ -1,23 +1,25 @@
+Require Import Program.
 Require Import Util.
 Require Export reduction_semantics.
+Require Import reduction_semantics_facts.
 Require Export refocusing_step.
 
 
 
 Module Type RED_REF_LANG.
 
-  Declare Module R   : RED_LANG.
-  Declare Module DEC : REF_STEP R.
-  Export R.
-  Export DEC.
+  Declare Module R  : RED_LANG.
+  Declare Module ST : STRATEGY_STEP R.
+  Export R ST.
 
 
   (* A property of deterministic reduction semantics: *)
-  Axiom redex_trivial : forall {k} (r : redex k), only_trivial r k.
+  Axiom redex_trivial1 : forall {k} (r : redex k) ec t, 
+                             ~dead_ckind (k+>ec) -> ec:[t] = r -> 
+                                 exists (v : value (k+>ec)), t = v.
 
 
-  Inductive subterm_one_step : term -> term -> Prop :=
-  | st_1 : forall {t t0} ec, t = ec:[t0] -> subterm_one_step t0 t.
+  Definition subterm_one_step t0 t := exists ec, t = ec:[t0].
   Axiom wf_st1 : well_founded subterm_one_step.
 
 
@@ -36,8 +38,8 @@ Module Type RED_REF_LANG.
   Axiom ec_order_trans   : forall k t ec0 ec1 ec2,
       k, t |~ ec0 << ec1 -> k, t |~ ec1 << ec2 -> k,t |~ ec0 << ec2.
 
-  Axiom ec_order_comp_if : forall t ec0 ec1,
-      immediate_ec ec0 t -> immediate_ec ec1 t -> 
+  Axiom ec_order_comp_if : 
+      forall t ec0 ec1, immediate_ec ec0 t -> immediate_ec ec1 t -> 
       forall k, ~ dead_ckind (k+>ec0) -> ~ dead_ckind (k+>ec1) ->
           k, t |~ ec0 << ec1  \/  k, t |~ ec1 << ec0  \/  ec0 = ec1.
 
@@ -80,13 +82,278 @@ End RED_REF_LANG.
 
 
 
+
+Module Type RED_REF_LANG_minus.
+
+  (* Inhered from RED_REF_LANG : *)
+
+  Declare Module SX : RED_SYNTAX.
+  Declare Module ST : STRATEGY_STEP SX.
+  Export SX ST.
+
+
+  Axiom death_propagation : 
+      forall k, dead_ckind k -> forall ec, dead_ckind (k+>ec).
+  Axiom proper_death : 
+      forall k, dead_ckind k -> ~ exists (r : redex k), True.
+
+
+  Parameter  init_ckind : ckind.
+
+
+  Axiom value_trivial1 : 
+      forall {k} (v : value k) ec t, 
+          ~dead_ckind (k+>ec) -> ec:[t] = v -> 
+              exists (v' : value (k+>ec)), t = v'.
+  Axiom value_redex    : forall {k} (v : value k) (r : redex k), 
+                             value_to_term v <> redex_to_term r.
+
+
+  Parameter contract : forall {k}, redex k -> option term.
+
+
+  Axiom redex_trivial1 : forall {k} (r : redex k) ec t, 
+                             ~dead_ckind (k+>ec) -> ec:[t] = r -> 
+                                 exists (v : value (k+>ec)), t = v.
+
+  Definition only_empty t k :=
+      forall t' {k'} (c : context k k'), c[t'] = t -> ~ dead_ckind k' -> 
+          k = k' /\ c ~= [.](k).
+  Definition only_trivial t k :=
+      forall t' {k'} (c : context k k'), c[t'] = t -> ~ dead_ckind k' -> 
+          k = k' /\ c ~= [.](k) \/ exists (v : value k'), t' = v.
+
+
+  Definition subterm_one_step t0 t := exists ec, t = ec:[t0].
+  Axiom wf_st1 : well_founded subterm_one_step.
+
+
+  Definition subterm_order := clos_trans_1n term subterm_one_step.
+  Notation "t1 <| t2" := (subterm_order t1 t2) (at level 40, no associativity).
+  Definition wf_sto : well_founded subterm_order := wf_clos_trans_l _ _ wf_st1.
+
+
+  Parameter ec_order : ckind -> term -> elem_context -> elem_context -> Prop.
+  Notation "k , t |~  ec1 << ec2 " := (ec_order k t ec1 ec2) (at level 40, no associativity).
+  Axiom wf_eco : forall k t, well_founded (ec_order k t).
+
+  Axiom ec_order_antisym : forall k t ec ec0, 
+      k, t |~ ec << ec0 -> ~ k, t |~ ec0 << ec.
+
+  Axiom ec_order_trans   : forall k t ec0 ec1 ec2,
+      k, t |~ ec0 << ec1 -> k, t |~ ec1 << ec2 -> k,t |~ ec0 << ec2.
+
+  Axiom ec_order_comp_if : forall t ec0 ec1,
+      immediate_ec ec0 t -> immediate_ec ec1 t -> 
+      forall k, ~ dead_ckind (k+>ec0) -> ~ dead_ckind (k+>ec1) ->
+          k, t |~ ec0 << ec1  \/  k, t |~ ec1 << ec0  \/  ec0 = ec1.
+
+  Axiom ec_order_comp_fi : forall k t ec0 ec1,
+      k, t |~ ec0 << ec1  ->  immediate_ec ec0 t /\ immediate_ec ec1 t /\ 
+                                  ~ dead_ckind (k+>ec0) /\ ~ dead_ckind (k+>ec1).
+
+
+
+  Axiom dec_term_red_empty : 
+      forall t k {r : redex k}, dec_term t k = in_red r -> only_empty t k.
+
+  Axiom dec_term_val_empty : 
+      forall t k {v : value k}, dec_term t k = in_val v -> only_empty t k.
+
+  Axiom dec_term_term_top : 
+      forall t k {t' ec}, dec_term t k = in_term t' ec -> 
+          forall ec',  ~ k, t |~ ec << ec'.
+
+  Axiom dec_context_red_bot : 
+      forall k ec v {r : redex k}, dec_context ec k v = in_red r -> 
+          forall ec',  ~ k, ec:[v] |~ ec' << ec.
+
+  Axiom dec_context_val_bot : 
+      forall k ec v {v' : value k}, dec_context ec k v = in_val v' -> 
+          forall ec',  ~ k, ec:[v] |~ ec' << ec.
+
+  Axiom dec_context_term_next : 
+      forall ec0 k v {t ec1}, dec_context ec0 k v = in_term t ec1 -> 
+      (*1*) k, ec0:[v] |~ ec1 << ec0 /\ 
+      (*2*) forall ec,  k, ec0:[v] |~ ec << ec0  ->  ~ k, ec0:[v] |~ ec1 << ec.
+
+
+  Axiom elem_context_det : 
+      forall t ec {t'}, t = ec:[t'] -> 
+          forall k ec',  k, t |~ ec' << ec -> 
+              exists (v : value (k+>ec)), t' = v.
+
+End RED_REF_LANG_minus.
+
+
+
+
+Module mk_RedRefLang (PR : RED_REF_LANG_minus) <: RED_REF_LANG.
+
+  Module SXF := RED_SYNTAX_Facts PR.SX.
+  Import SXF.
+
+
+  Module R <: RED_LANG.
+
+    Include PR.SX.
+
+    Definition death_propagation : 
+        forall k, dead_ckind k -> forall ec, dead_ckind (k+>ec)
+
+        := PR.death_propagation.
+
+    Definition proper_death : 
+        forall k, dead_ckind k -> ~ exists (r : redex k), True
+
+        := PR.proper_death.
+
+    Definition only_empty t k :=
+        forall t' {k'} (c : context k k'), c[t'] = t -> ~ dead_ckind k' -> 
+            k = k' /\ c ~= [.](k).
+    Definition only_trivial t k :=
+        forall t' {k'} (c : context k k'), c[t'] = t -> ~ dead_ckind k' -> 
+            k = k' /\ c ~= [.](k) \/ exists (v : value k'), t' = v.
+
+    Definition value_trivial1 : 
+        forall {k} (v : value k) ec t, 
+            ~dead_ckind (k+>ec) -> ec:[t] = v -> 
+                exists (v' : value (k+>ec)), t = v'
+
+        := @PR.value_trivial1.
+    Definition value_redex   : forall {k} (v : value k) (r : redex k), 
+                            value_to_term v <> redex_to_term r
+        := @PR.value_redex.
+
+
+    Lemma decompose : 
+        forall (t : term) k1, ~ dead_ckind k1 ->
+            (exists (v : value k1), t = v) \/
+            (exists k2 (r : redex k2) (c : context k1 k2), t = c[r]).
+
+    Proof with eauto.
+      induction t using (well_founded_ind PR.wf_sto); intros.
+
+      remember (PR.ST.dec_term t k1); assert (hh := PR.ST.dec_term_correct t k1);
+      symmetry in Heqi;
+      destruct i; rewrite Heqi in hh.
+
+      - right; exists k1; exists r; eexists [.]...
+
+      - destruct (H t0) with (k1 := k1+>e) as [(v, Hv) | (k2, (r, (c, Hrc)))].
+            repeat econstructor...
+            eapply PR.ST.dec_term_next_alive... 
+
+        + { subst t0.
+          assert (~ dead_ckind (k1+>e)) as Hndk.
+            { eapply PR.ST.dec_term_next_alive... } 
+          clear Heqi; generalize dependent v.
+          induction e using (well_founded_ind (PR.wf_eco k1 t)); intros.
+
+          remember (PR.ST.dec_context e _ v); assert (ht := PR.ST.dec_context_correct e _ v); 
+          destruct i; rewrite <- Heqi in ht; try 
+          (   compute in hh; rewrite <- hh in ht).
+
+          - right; exists k1; exists r; eexists [.]...
+
+          - destruct (H t0) with (k1 := k1+>e0) as [(v0, Hv) | (k2, (r, (c, Hrc)))].
+                repeat econstructor...
+                eapply PR.ST.dec_context_next_alive...
+
+            + symmetry in Heqi.
+              destruct (PR.dec_context_term_next _ _ _ Heqi) as (H2, _).
+
+              subst t0.
+              assert (~ dead_ckind (k1+>e0)) as Hndk2.
+                { eapply PR.ST.dec_context_next_alive... }
+              rewrite <- hh in H2.
+              destruct (H1 e0 H2 Hndk2 v0 ht) as [(v1, Hv1) | (k2, (r, (c, Hrc)))].
+              * left; exists v1...
+              * right; exists k2; exists r; exists c...
+
+            + right; exists k2; exists r; exists (c~+e0=:[.]).
+              subst t0; rewrite plug_compose...
+
+          - left; exists v0...
+
+          - intuition. 
+          }
+
+        + right; exists k2; exists r; exists (c~+(e=:[.])).
+          subst t0; rewrite plug_compose...
+
+      - left; exists v...
+
+      - intuition.
+    Qed. 
+
+    Inductive decomp k : Set :=
+    | d_red : forall {k'}, redex k' -> context k k' -> decomp k
+    | d_val : value k -> decomp k.
+    Arguments d_val {k} _. Arguments d_red {k} {k'} _ _.
+
+
+    Definition decomp_to_term {k} (d : decomp k) :=
+        match d with
+        | d_val v     => value_to_term v
+        | d_red _ r c => c[r]
+        end.
+    Coercion decomp_to_term : decomp >-> term.
+
+
+    Definition contract {k} r := @PR.contract k r.
+
+    Definition init_ckind := PR.init_ckind.
+
+  End R.
+
+
+  Module ST := PR.ST.
+
+  Export R ST.
+
+  Definition redex_trivial1 {k} := @PR.redex_trivial1 k.
+  Definition subterm_one_step t0 t := exists ec, t = ec:[t0].
+  Definition wf_st1 := PR.wf_st1.
+
+
+  Definition subterm_order := clos_trans_1n term subterm_one_step.
+  Notation "t1 <| t2" := (subterm_order t1 t2) (at level 40, no associativity).
+  Definition wf_sto := wf_clos_trans_l _ _ wf_st1.
+
+
+  Definition ec_order := PR.ec_order.
+  Notation "k , t |~  ec1 << ec2 " := (ec_order k t ec1 ec2) (at level 40, no associativity).
+  Definition wf_eco := PR.wf_eco.
+
+  Definition ec_order_antisym := PR.ec_order_antisym.
+  Definition ec_order_trans   := PR.ec_order_trans.
+  Definition ec_order_comp_if := PR.ec_order_comp_if.
+  Definition ec_order_comp_fi := PR.ec_order_comp_fi.
+
+
+  Definition dec_term_red_empty := PR.dec_term_red_empty.
+  Definition dec_term_val_empty := PR.dec_term_val_empty.
+  Definition dec_term_term_top  := PR.dec_term_term_top.
+
+  Definition dec_context_red_bot   := PR.dec_context_red_bot.
+  Definition dec_context_val_bot   := PR.dec_context_val_bot.
+  Definition dec_context_term_next := PR.dec_context_term_next.
+
+
+  Definition elem_context_det := PR.elem_context_det.
+
+End mk_RedRefLang.
+
+
+
 Module RED_REF_LANG_Help.
 
   Ltac prove_st_wf := 
       intro t; constructor; induction t; 
       (
           intros ? H; 
-          inversion H as [? ? ec DECT]; subst; 
+          inversion H as [ec DECT]; subst; 
           destruct ec; inversion DECT; subst; 
           constructor; auto
       ).
